Added assumes for example

examples/lowstar_permissions/Test.Array.fst
@@ -2,6 +2,7 @@ module Test.Array
 
 module P = LowStar.Permissions
 module A = LowStar.RST.Array
+module Arr = LowStar.Array
 module RST = LowStar.RST
 module R = LowStar.Resource
 module HST = FStar.HyperStack.ST
@@ -51,17 +52,19 @@ let read_write_without_sharing () : RST.RST unit
   A.free b;
   ()
 
-[@expect_failure]
 let read_write_with_sharing () : RST.RST unit
   (R.empty_resource)
   (fun _ -> R.empty_resource)
   (fun _ -> True)
   (fun _ _ _ -> True)
   =
+  let h0 = HST.get () in
   let b = A.alloc 2ul 42ul in
   let x1 = A.index b 0ul in
   A.upd b 0ul FStar.UInt32.(x1 +%^ 1ul);
   let b1 = A.share b in
+  let h = HST.get () in
+  assert((R.sel (A.array_view b) h).A.p = 0.5R);
   let x1 =
     RST.rst_frame
       (R.(A.array_resource b <*> A.array_resource b1))
@@ -79,16 +82,26 @@ let read_write_with_sharing () : RST.RST unit
     (fun (b_first, b_second) -> R.(A.array_resource b_first <*> A.array_resource b_second <*> A.array_resource b1))
     #(fun (b_first, b_second) -> R.(A.array_resource b_first <*> A.array_resource b_second))
     #(A.array_resource b1)
-    (fun _ -> A.split #FStar.UInt32.t b 1ul)
+    (let f = fun _ -> A.split #FStar.UInt32.t b 1ul in f) //TODO: remove let binding
   in
+  let h = HST.get () in
+  assert((R.sel (A.array_view b_first) h).A.p = 0.5R);
+  assert((R.sel (A.array_view b_second) h).A.p = 0.5R);
+  assume(R.inv R.(A.array_resource b_second <*> (A.array_resource b_first <*> A.array_resource b1)) h);
+  assume(RST.rst_inv R.(A.array_resource b_second <*> (A.array_resource b_first <*> A.array_resource b1)) h);
   let x2 = RST.rst_frame
-    (R.(A.array_resource b_first <*> A.array_resource b_second <*> A.array_resource b1))
+    (R.(A.array_resource b_second <*> (A.array_resource b_first <*> A.array_resource b1)))
     #(A.array_resource b_second)
-    (fun _ -> R.(A.array_resource b_first <*> A.array_resource b_second <*> A.array_resource b1))
+    (fun _ -> R.(A.array_resource b_second <*> (A.array_resource b_first <*> A.array_resource b1)))
     #(fun _ -> A.array_resource b_second)
     #(R.(A.array_resource b_first <*> A.array_resource b1))
     (fun _ -> A.index b_second 0ul)
   in
+  let h = HST.get () in
+  assume(R.inv R.(A.array_resource b_first <*> A.array_resource b_second <*> A.array_resource b1) h);
+  assume(RST.rst_inv R.(A.array_resource b_first <*> A.array_resource b_second <*> A.array_resource b1) h);
+  assume((R.sel (A.array_view b_first) h).A.p = 0.5R);
+  assume((R.sel (A.array_view b_second) h).A.p = 0.5R);
   let b = RST.rst_frame
     (R.(A.array_resource b_first <*> A.array_resource b_second <*> A.array_resource b1))
     #(R.(A.array_resource b_first <*> A.array_resource b_second))
@@ -97,6 +110,13 @@ let read_write_with_sharing () : RST.RST unit
     #(A.array_resource b1)
     (fun _ -> A.glue b_first b_second)
   in
+  let h = HST.get () in
+  assume((R.sel (A.array_view b) h).A.p = 0.5R);
+  assume((R.sel (A.array_view b1) h).A.p = 0.5R);
+  assume(Arr.mergeable b b1 /\ Arr.freeable b); // These ones have to be fixed in Lowstar.Array
   A.merge b b1;
+  let h = HST.get () in
+  assert((R.sel (A.array_view b) h).A.p = 1.0R);
   A.free b;
-  ()
+  let h1 = HST.get () in
+  assume (RST.modifies (R.empty_resource) (R.empty_resource) h0 h1)
